NewEchoAll to asm proof

examples/new_echo/NewEchoAll.v
@@ -1,17 +1,12 @@
-Require Import Coqlib.
-Require Import ITreelib.
-Require Import ImpPrelude.
-Require Import STS.
-Require Import Behavior.
-Require Import ModSem.
-Require Import Skeleton.
-Require Import PCM.
-Require Import Hoare.
-Require Import MutHeader SimModSem.
-Require Import OpenDef.
-Require Import Mem0 NewStack3A NewStack0 NewEcho0 NewEchoMain0 NewClient0.
+Require Import Coqlib ITreelib ImpPrelude STS Behavior.
+Require Import ModSem Skeleton PCM STB OpenDef.
+Require Import SimModSem Open.
+Require Import Mem0 Mem1 NewStack3A.
+Require Import Imp NewStackImp NewEchoImp NewEchoMainImp NewClientImp.
 
 Set Implicit Arguments.
+
+
 
 
 Definition EchoGRA: GRA.t := GRA.of_list [Mem1.memRA; stkRA].
@@ -30,67 +25,52 @@ Qed.
 Local Existing Instance stkRA_inG.
 
 
-
-Section ECHOIMPL.
-  Definition echo_impl: ModL.t :=
-    Mod.add_list [Mem; Stack; Echo; Main; Client].
-  Definition echo_impl_itr := ModSemL.initial_itr (ModL.enclose echo_impl) None.
-End ECHOIMPL.
-
-
+(* Imp program *)
 Require Import Mem0 NewStackImp NewEchoImp NewEchoMainImp NewClientImp.
 Section ECHOIMP.
+  Definition echo_progs := [Stack_prog; Echo_prog; EchoMain_prog; Client_prog].
   Definition echo_imp: ModL.t :=
-    Mod.add_list [Mem; Stack; Echo; EchoMain; Client].
+    Mod.add_list (Mem :: map ImpMod.get_mod echo_progs).
+
   Definition echo_imp_itr := ModSemL.initial_itr (ModL.enclose echo_imp) None.
 End ECHOIMP.
 
 
+Require Import Mem0 NewStack0 NewEcho0 NewEchoMain0 NewClient0.
+Section ECHOIMPL.
+  Definition echo_impl: ModL.t :=
+    Mod.add_list [Mem; Stack; Echo; Main; Client].
+
+  Definition echo_impl_itr := ModSemL.initial_itr (ModL.enclose echo_impl) None.
+End ECHOIMPL.
+
+
+(* spec program *)
 Require Import MemOpen NewStack3A NewEcho1 NewEchoMain0 NewClient0.
 Section ECHOSPEC.
   Let frds: list string := ["Stack"; "Echo"].
   Definition echo_spec: ModL.t :=
     Mod.add_list [
-      Mem0.Mem;
-      (KMod.transl_src (fun _ => frds) KStack);
-      (KMod.transl_src (fun _ => frds) KEcho);
-      Main;
-      Client
+        Mem0.Mem;
+      KMod.transl_src (fun _ => frds) KStack; KMod.transl_src (fun _ => frds) KEcho;
+      Main; Client
       ].
 
   Definition echo_spec_itr := ModSemL.initial_itr (ModL.enclose echo_spec) None.
 End ECHOSPEC.
 
 
-Lemma refines2_cons mhd0 mhd1 mtl0 mtl1
-      (HD: refines2 [mhd0] [mhd1])
-      (TL: refines2 mtl0 mtl1)
-  :
-    refines2 (mhd0::mtl0) (mhd1::mtl1).
-Proof.
-Admitted.
-
-Lemma refines2_app mhd0 mhd1 mtl0 mtl1
-      (HD: refines2 mhd0 mhd1)
-      (TL: refines2 mtl0 mtl1)
-  :
-    refines2 (mhd0++mtl0) (mhd1++mtl1).
-Proof.
-Admitted.
-
-Require Import NewEchoMainImp0proof NewStackImp0proof NewEchoImp0proof NewClientImp0proof NewStack01proof NewStack12proof NewStack23Aproof NewEcho01proof.
-Require Import SimModSem.
 Require Import Mem0Openproof MemOpen0proof.
-Require Import Open.
-
-
+Require Import NewStackImp0proof NewStack01proof NewStack12proof NewStack23Aproof.
+Require Import NewEchoMainImp0proof NewEchoImp0proof.
+Require Import NewClientImp0proof  NewEcho01proof.
 Section PROOF.
   Theorem echo_correct:
     refines echo_imp echo_spec.
   Proof.
     unfold echo_imp, echo_spec. transitivity echo_impl.
     { eapply refines2_pairwise. econs.
-      { ss. }
+      { cbn. ss. }
       econs.
       { eapply adequacy_local2. eapply NewStackImp0proof.correct. }
       econs.
@@ -138,5 +118,24 @@ Section PROOF.
     eapply adequacy_open. i. exists ε. split.
     { admit "URA wf". }
     { ii. ss. }
+  Qed.
+End PROOF.
+
+
+Require Import SimSTS2 Imp2Csharpminor Imp2Asm.
+Require Import Imp2AsmProof.
+Section PROOF.
+  Context `{builtins : builtinsTy}.
+  Hypothesis source_linking: exists impl, link_imps echo_progs = Some impl.
+
+  Theorem echo_compile_correct
+          (asms : Coqlib.nlist Asm.program)
+          (COMP: Forall2 (fun imp asm => compile_imp imp = Errors.OK asm) echo_progs asms)
+    :
+      exists asml, (Linking.link_list asms = Some asml) /\
+                   (improves2_program (ModL.compile echo_spec) (Asm.semantics asml)).
+  Proof.
+    hexploit compile_behavior_improves; [et|et|]. i. des. esplits; [et|].
+    eapply improves_combine; [|et]. eapply refines_close. eapply echo_correct.
   Qed.
 End PROOF.
